Spacetalk/DotProduct.lean
@@ -1,0 +1,25 @@
+import Spacetalk.Step
+import Spacetalk.VirtualRDA
+
+
+def dot_prod (n : Nat) (a : Stream' Nat) (b : Stream' Nat) : Stream' Nat :=
+  Stream'.reduce (· + ·) n 0 (Stream'.zip (· * ·) a b)
+
+namespace Step
+  -- A dot product of length n vectors
+  def dot_prod (n : Nat) : Prog rep (.stream .nat → .stream .nat → .stream .nat) :=
+    let multiply := .zip (.binop .mul)
+    let reduction := .reduce (.binop .add) n 0
+    .lam λ a => .lam λ b => .app reduction (.app (.app multiply (.var a)) (.var b))
+
+  def sa : Stream' Nat := id
+  def sb : Stream' Nat := id
+
+  def dp (n : Nat) := (dot_prod n).denote sa sb
+  def n := 10
+  #eval (dp n).get 0
+
+end Step
+
+theorem step_dp_equiv : ∀n : Nat, (Step.dot_prod n).denote = dot_prod n := by
+  simp [dot_prod]
